Switch to result monads in FA1.2 contract

examples/fa1_2/FA1_2.v
@@ -6,6 +6,7 @@ From ConCert.Utils Require Import RecordUpdate.
 From ConCert.Execution Require Import Blockchain.
 From ConCert.Execution Require Import Containers.
 From ConCert.Execution Require Import Monads.
+From ConCert.Execution Require Import ResultMonad.
 From ConCert.Execution Require Import Serializable.
 From ConCert.Execution Require Import ContractCommon.
 From Coq Require Import ZArith_base.
@@ -205,40 +206,48 @@ Definition empty_allowance : FMap (Address * Address) N := FMap.empty.
 (** ** Transfer *)
 (** Transfers [amount] tokens, if [from] has enough tokens to transfer
     and [sender] is allowed to send that much on behalf of [from] *)
-Definition try_transfer (sender : Address) (param : transfer_param) (state : State) : option State :=
+Definition try_transfer (sender : Address)
+                        (param : transfer_param)
+                        (state : State)
+                        : result State unit :=
   let allowances_ := state.(allowances) in
   let tokens_ := state.(tokens) in
   do allowances_ <- (* Update allowances *)
     (if address_eqb sender param.(from)
-    then Some allowances_
+    then Ok allowances_
     else
       let allowance_key := (param.(from), sender) in
       let authorized_value := with_default 0 (find_allowance allowance_key allowances_) in
-        do _ <- throwIf (authorized_value <? param.(value)) ; (* NotEnoughAllowance *)
-        Some (update_allowance allowance_key (maybe (authorized_value - param.(value))) allowances_)
+        do _ <- throwIf (authorized_value <? param.(value)) tt; (* NotEnoughAllowance *)
+        Ok (update_allowance allowance_key (maybe (authorized_value - param.(value))) allowances_)
     ) ;
   do tokens_ <- (* Update from balance *)
     (let from_balance := with_default 0 (AddressMap.find param.(from) tokens_) in
-      do _ <- throwIf (from_balance <? param.(value)) ; (* NotEnoughBalance *)
-      Some (AddressMap.update param.(from) (maybe (from_balance - param.(value))) tokens_)
+      do _ <- throwIf (from_balance <? param.(value)) tt; (* NotEnoughBalance *)
+      Ok (AddressMap.update param.(from) (maybe (from_balance - param.(value))) tokens_)
     ) ;
   let tokens_ :=
     let to_balance := with_default 0 (AddressMap.find param.(to) tokens_) in
       AddressMap.update param.(to) (maybe (to_balance + param.(value))) tokens_ in
-    Some (state<|tokens := tokens_|>
+    Ok (state<|tokens := tokens_|>
                <|allowances := allowances_|>).
 
 (** ** Approve *)
 (** The caller approves the [spender] to transfer up to [amount] tokens on behalf of the [sender] *)
-Definition try_approve (sender : Address) (param : approve_param) (state : State) : option State :=
+Definition try_approve (sender : Address)
+                       (param : approve_param)
+                       (state : State)
+                       : result State unit :=
   let allowances_ := state.(allowances) in
   let allowance_key := (sender, param.(spender)) in
   let previous_value := with_default 0 (find_allowance allowance_key allowances_) in
-  do _ <- throwIf (andb (0 <? previous_value) (0 <? param.(value_))) ; (* UnsafeAllowanceChange *)
+  do _ <- throwIf (andb (0 <? previous_value) (0 <? param.(value_))) tt; (* UnsafeAllowanceChange *)
   let allowances_ := update_allowance allowance_key (maybe param.(value_)) allowances_ in
-    Some (state<|allowances := allowances_|>).
+    Ok (state<|allowances := allowances_|>).
 
-Definition mk_callback (to_addr : Address) (msg : @FA12ReceiverMsg unit) :=
+Definition mk_callback (to_addr : Address)
+                       (msg : @FA12ReceiverMsg unit)
+                       : ActionBody :=
   act_call to_addr 0 (serialize msg).
 
 Definition receive_allowance_ n := @receive_allowance unit n.
@@ -247,27 +256,39 @@ Definition receive_total_supply_ n := @receive_total_supply unit n.
 
 (** ** Get allowance *)
 (** Get the quantity that [snd request] is allowed to spend on behalf of [fst request] *)
-Definition try_get_allowance (sender : Address) (param : getAllowance_param) (state : State) : list ActionBody :=
+Definition try_get_allowance (sender : Address)
+                             (param : getAllowance_param)
+                             (state : State)
+                             : list ActionBody :=
   let value := with_default 0 (find_allowance param.(request) state.(allowances)) in
     [mk_callback param.(allowance_callback) (receive_allowance_ value)].
 
 (** ** Get balance *)
 (** Get the quantity of tokens belonging to [owner] *)
-Definition try_get_balance (sender : Address) (param : getBalance_param) (state : State) : list ActionBody :=
+Definition try_get_balance (sender : Address)
+                           (param : getBalance_param)
+                           (state : State)
+                           : list ActionBody :=
   let value := with_default 0 (AddressMap.find param.(owner_) state.(tokens)) in
     [mk_callback param.(balance_callback) (receive_balance_of_ value)].
 
 (** ** Get total supply *)
 (** Get the total supply of tokens *)
-Definition try_get_total_supply (sender : Address) (param : getTotalSupply_param) (state : State) : list ActionBody :=
+Definition try_get_total_supply (sender : Address)
+                                (param : getTotalSupply_param)
+                                (state : State)
+                                : list ActionBody :=
   let value := state.(total_supply) in
     [mk_callback param.(supply_callback) (receive_total_supply_ value)].
 
 (** ** Init *)
 (** Initalize contract storage *)
-Definition init (chain : Chain) (ctx : ContractCallContext) (setup : Setup) : option State :=
-  do _ <- throwIf (non_zero_amount ctx.(ctx_amount)); (* DontSendTez *)
-  Some {|
+Definition init (chain : Chain)
+                (ctx : ContractCallContext)
+                (setup : Setup)
+                : result State unit :=
+  do _ <- throwIf (non_zero_amount ctx.(ctx_amount)) tt; (* DontSendTez *)
+  Ok {|
     tokens := AddressMap.add setup.(lqt_provider) setup.(initial_pool) AddressMap.empty;
     allowances := empty_allowance;
     total_supply := setup.(initial_pool);
@@ -276,24 +297,26 @@ Definition init (chain : Chain) (ctx : ContractCallContext) (setup : Setup) : op
 (** ** Receive *)
 (** Contract main entrypoint *)
 Open Scope Z_scope.
-Definition receive (chain : Chain) (ctx : ContractCallContext)
-                   (state : State) (maybe_msg : option Msg)
-                    : option (State * list ActionBody) :=
+Definition receive (chain : Chain)
+                   (ctx : ContractCallContext)
+                   (state : State)
+                   (maybe_msg : option Msg)
+                   : result (State * list ActionBody) unit :=
   let sender := ctx.(ctx_from) in
-  let without_actions := option_map (fun new_state => (new_state, [])) in
-  let without_statechange acts := Some (state, acts) in
-  do _ <- throwIf (non_zero_amount ctx.(ctx_amount)); (* DontSendTez *)
+  let without_actions x := x >>= (fun new_state => Ok (new_state, [])) in
+  let without_statechange acts := Ok (state, acts) in
+  do _ <- throwIf (non_zero_amount ctx.(ctx_amount)) tt; (* DontSendTez *)
   match maybe_msg with
   | Some (transfer param) => without_actions (try_transfer sender param state)
   | Some (approve param) => without_actions (try_approve sender param state)
   | Some (getAllowance param) => without_statechange (try_get_allowance sender param state)
   | Some (getBalance param) => without_statechange (try_get_balance sender param state)
   | Some (getTotalSupply param) => without_statechange (try_get_total_supply sender param state)
-  | None => None (* Transfer actions to this contract are not allowed *)
+  | None => Err tt (* Transfer actions to this contract are not allowed *)
   end.
 Close Scope Z_scope.
 
-Definition contract : Contract Setup Msg State :=
+Definition contract : Contract Setup Msg State unit :=
   build_contract init receive.
 
   End FA12Defs.
